WIP on fuel-free stepping list.

src/BinEncoders/Env/Common/Transformer.v
@@ -3,6 +3,10 @@ Set Implicit Arguments.
 Class Transformer (bin : Type) :=
   { transform : bin -> bin -> bin;
     transform_id : bin;
+    bin_measure : bin -> nat;
+    transform_measure :
+      forall b b', bin_measure (transform b b') =
+                   bin_measure b + bin_measure b';
     transform_id_left : forall l, transform transform_id l = l;
     transform_id_right : forall l, transform l transform_id = l;
     transform_assoc : forall l m n, transform l (transform m n) = transform (transform l m) n }.
@@ -15,15 +19,42 @@ Class TransformerUnit (bin : Type) (trans : Transformer bin) (T : Type) :=
                                         transform_push t (transform m n) }.
 
 Class TransformerUnitOpt (bin : Type) (trans : Transformer bin) (T : Type) :=
-  { transform_push_opt : T -> bin -> bin;
+  { T_measure : T -> nat;
+    transform_push_opt : T -> bin -> bin;
     transform_pop_opt : bin -> option (T * bin);
+    measure_push :
+      forall t b,
+        bin_measure (transform_push_opt t b) = bin_measure b + T_measure t;
+    measure_pop_Some :
+      forall b' t b,
+        transform_pop_opt b = Some (t, b')
+        -> bin_measure b = bin_measure b' + T_measure t;
     transform_push_pop_opt :
       forall t m, transform_pop_opt (transform_push_opt t m) = Some (t, m);
-    transform_push_step_opt : forall t m n, transform (transform_push_opt t m) n =
-                                            transform_push_opt t (transform m n);
+    transform_push_step_opt
+    : forall t m n, transform (transform_push_opt t m) n =
+                    transform_push_opt t (transform m n);
     transform_pop_opt_inj :
       forall t m b b',
         transform_pop_opt b = Some (t, m) ->
         transform_pop_opt b' = Some (t, m) ->
         b = b'
   }.
+
+  Definition lt_B {B} {transformer : Transformer B} (b b' : B) : Prop :=
+    bin_measure b < bin_measure b'.
+
+  Definition le_B {B} {transformer : Transformer B} (b b' : B) : Prop :=
+    bin_measure b <= bin_measure b'.
+
+  Lemma well_founded_lt_b {B}
+        {transformer : Transformer B}
+    : well_founded lt_B.
+  Proof.
+    constructor.
+    unfold lt_B; induction (bin_measure a); intros.
+    - inversion H.
+    - inversion H; subst.
+      + constructor; eauto.
+      + eauto.
+  Qed.
